Working test

InfoviewSearch/Util.lean
@@ -172,28 +172,33 @@ end Syntax
 
 section Widget
 
-def mkSuggestion (tac : TSyntax `tactic) (pasteInfo : PasteInfo)
-    (html : Html) (isText := false) : CoreM Html := do
+def createTacticInsertionEdit (tac : TSyntax `tactic) (pasteInfo : PasteInfo) :
+    CoreM Lsp.TextEdit := do
   let singleTactic ← tacticPasteString tac pasteInfo
-  let (tactic, replaceRange) ← (do
-    if let some range := pasteInfo.stx.getRange? then
+  if let some range := pasteInfo.stx.getRange? then
       let text := pasteInfo.meta.text
       if let some tac ← mergeTactics? pasteInfo.stx tac then
         let endPos := max (text.lspPosToUtf8Pos pasteInfo.cursorPos) range.stop
         let extraWhitespace := range.stop.extract text.source endPos
         let tactic ← tacticPasteString tac pasteInfo
-        return (tactic ++ extraWhitespace, text.utf8RangeToLspRange ⟨range.start, endPos⟩)
+        return {  newText := tactic ++ extraWhitespace,
+                  range   := text.utf8RangeToLspRange ⟨range.start, endPos⟩  }
       else
         let indent := text.utf8PosToLspPos range.start |>.character
-        return (s!"\n{String.replicate indent ' '}{singleTactic}",
-          text.utf8RangeToLspRange ⟨range.stop, range.stop⟩)
-    return (s!"{singleTactic}\n{String.replicate pasteInfo.cursorPos.character ' '}",
-      ⟨pasteInfo.cursorPos, pasteInfo.cursorPos⟩))
+        return {  newText := s!"\n{String.replicate indent ' '}{singleTactic}",
+                  range   := text.utf8RangeToLspRange ⟨range.stop, range.stop⟩  }
+    return {  newText := s!"{singleTactic}\n{String.replicate pasteInfo.cursorPos.character ' '}",
+              range   := ⟨pasteInfo.cursorPos, pasteInfo.cursorPos⟩  }
+
+def mkSuggestion (tac : TSyntax `tactic) (pasteInfo : PasteInfo)
+    (html : Html) (isText := false) : CoreM Html := do
+  let singleTactic ← tacticPasteString tac pasteInfo
+  let edit ← createTacticInsertionEdit tac pasteInfo
   let button :=
     -- TODO: The hover on this button should be a `CodeWithInfos`, instead of a string.
     <span className="font-code"> {
       Html.ofComponent MakeEditLink
-        (.ofReplaceRange pasteInfo.meta replaceRange tactic)
+        (.ofReplaceRange pasteInfo.meta edit.range edit.newText)
         #[<a
           className={"mh2 codicon codicon-insert"}
           style={json% { "position" : "relative", "top" : "0.15em"}}
